big step semantics

Cslib/Languages/Imp/OpSem/BigStep.lean
@@ -5,11 +5,109 @@ Authors: Tanner Duve
 -/
 
 import Cslib.Languages.Imp.Syntax
+import Aesop
 
 /-!
 # Big-step Operational Semantics for IMP
 
-This file defines the big-step operational semantics for IMP.
+This file defines and proves determinism of the big-step operational semantics for IMP.
+
+## References
+
+- [Pierce et al., *Software Foundations*][PierceEtAl2025]
+- [Baanen et al., *The Hitchhiker's Guide to Logical Verification*][BaanenEtAl2018]
 -/
 
 namespace Imp
+
+open Function
+
+/--
+Evaluate an arithmetic expression in a given state.
+-/
+def aexp_eval (st : State) (a : aexp) : Val :=
+  match a with
+  | aexp.ANum n => n
+  | aexp.AId x => st x
+  | aexp.APlus a1 a2 => aexp_eval st a1 + aexp_eval st a2
+  | aexp.AMinus a1 a2 => aexp_eval st a1 - aexp_eval st a2
+  | aexp.AMult a1 a2 => aexp_eval st a1 * aexp_eval st a2
+
+/--
+Evaluate a boolean expression in a given state.
+-/
+def bexp_eval (st : State) (b : bexp) : Prop :=
+  match b with
+  | bexp.BTrue => True
+  | bexp.BFalse => False
+  | bexp.BEq a1 a2 => aexp_eval st a1 = aexp_eval st a2
+  | bexp.BNeq a1 a2 => aexp_eval st a1 ≠ aexp_eval st a2
+  | bexp.BLe a1 a2 => aexp_eval st a1 ≤ aexp_eval st a2
+  | bexp.BGt a1 a2 => aexp_eval st a1 > aexp_eval st a2
+  | bexp.BNot b => ¬ bexp_eval st b
+  | bexp.BAnd b1 b2 => bexp_eval st b1 ∧ bexp_eval st b2
+
+/--
+Big-step operational semantics for IMP
+-/
+inductive BigStep : Stmt × State → State → Prop where
+| Bskip (s) :
+  BigStep (Stmt.Cskip, s) s
+| Bassign (x a s) :
+  BigStep (Stmt.Cassign x a, s) (update s x (aexp_eval s a))
+| Bseq (S T s t u) (hS : BigStep (S, s) t) (hT : BigStep (T, t) u) :
+  BigStep (Stmt.Cseq S T, s) u
+| Bif_true (B S T s t) (hcond : bexp_eval s B) (hbody : BigStep (S, s) t) :
+  BigStep (Stmt.CifThenElse B S T, s) t
+| Bif_false (B S T s t) (hcond : ¬ bexp_eval s B) (hbody : BigStep (T, s) t) :
+  BigStep (Stmt.CifThenElse B S T, s) t
+| Bwhile_true (B S s t u) (hcond : bexp_eval s B) (hbody : BigStep (S, s) t)
+  (hrest : BigStep (Stmt.CwhileDo B S, t) u) :
+  BigStep (Stmt.CwhileDo B S, s) u
+| Bwhile_false (B S s) (hcond : ¬ bexp_eval s B) :
+  BigStep (Stmt.CwhileDo B S, s) s
+infix:110 " ⟹ " => BigStep
+
+/--
+The big-step operational semantics for IMP is deterministic.
+-/
+theorem BigStep_deterministic {Ss l r} (hl : Ss ⟹ l)
+      (hr : Ss ⟹ r) :
+    l = r :=
+  by
+    induction hl generalizing r with
+    | Bskip s =>
+      cases hr with
+      | Bskip => rfl
+    | Bassign x a s =>
+      cases hr with
+      | Bassign => rfl
+    | Bseq S T s l₀ l hS hT ihS ihT =>
+      cases hr with
+      | Bseq _ _ _ r₀ _ hS' hT' =>
+        cases ihS hS' with
+        | refl =>
+          cases ihT hT' with
+          | refl => rfl
+    | Bif_true B S T s l hB hS ih =>
+      cases hr with
+      | Bif_true _ _ _ _ _ hB' hS'  => apply ih hS'
+      | Bif_false _ _ _ _ _ hB' hS' => aesop
+    | Bif_false B S T s l hB hT ih =>
+      cases hr with
+      | Bif_true _ _ _ _ _ hB' hS'  => aesop
+      | Bif_false _ _ _ _ _ hB' hS' => apply ih hS'
+    | Bwhile_true B S s l₀ l hB hS hw ihS ihw =>
+      cases hr with
+      | Bwhile_true _ _ _ r₀ hB' hB' hS' hw' =>
+        cases ihS hS' with
+        | refl =>
+          cases ihw hw' with
+          | refl => rfl
+      | Bwhile_false _ _ _ hB' => aesop
+    | Bwhile_false B S s hB =>
+      cases hr with
+      | Bwhile_true _ _ _ s' _ hB' hS hw => aesop
+      | Bwhile_false _ _ _ hB'           => rfl
+
+end Imp
