CslibTests/ImpBigStep.lean
@@ -1,0 +1,28 @@
+import Cslib.Languages.Imp.OpSem.BigStep
+
+open Imp
+
+-- Examples using SF notation
+
+def plus2 : Stmt :=
+  <{ X := X + 2 }>
+
+def XtimesYinZ : Stmt :=
+  <{ Z := X × Y }>
+
+lemma plus2_spec
+  (st st' : State) (n : ℤ)
+  (hX : st "X" = n)
+  (hev : (plus2, st) ⟹ st') :
+  st' "X" = n + 2 := by
+  cases hev
+  simp [aexp_eval, hX]
+
+lemma XtimesYinZ_spec
+  (st st' : State) (n m : ℤ)
+  (hX : st "X" = n)
+  (hY : st "Y" = m)
+  (hev : (XtimesYinZ, st) ⟹ st') :
+  st' "Z" = n * m := by
+  cases hev
+  simp [aexp_eval, hX, hY]
